\begin{footnotesize}
\fbox{
	\parbox{26cm}{
\mbox{\vbox to 11pt{  \hbox{\textbf {Integrals of Rational Functions} }  }}
\
\mbox{\vbox to 11pt{  \hbox{$
\int \frac{1}{1+x^2}dx = \tan^{-1}x
$}  }}
\
\mbox{\vbox to 11pt{  \hbox{$
\int \frac{1}{a^2+x^2}dx = \frac{1}{a}\tan^{-1}\frac{x}{a}
$}  }}
\
\mbox{\vbox to 11pt{  \hbox{$
\int \frac{x}{a^2+x^2}dx = \frac{1}{2}\ln|a^2+x^2|
$}  }}
\
\mbox{\vbox to 11pt{  \hbox{$
\int \frac{x^2}{a^2+x^2}dx = x-a\tan^{-1}\frac{x}{a}
$}  }}
\
\mbox{\vbox to 11pt{  \hbox{$
\int \frac{x^3}{a^2+x^2}dx = \frac{1}{2}x^2-\frac{1}{2}a^2\ln|a^2+x^2|
$}  }}
\
\mbox{\vbox to 11pt{  \hbox{$
\int \frac{1}{ax^2+bx+c}dx = \frac{2}{\sqrt{4ac-b^2}}\tan^{-1}\frac{2ax+b}{\sqrt{4ac-b^2}}
$}  }}
\
\mbox{\vbox to 11pt{  \hbox{$
\int \frac{1}{(x+a)(x+b)}dx = \frac{1}{b-a}\ln\frac{a+x}{b+x}, \text{ } a\ne b
$}  }}
\
\mbox{\vbox to 11pt{  \hbox{$
\int \frac{x}{(x+a)^2}dx = \frac{a}{a+x}+\ln |a+x|
$}  }}
\
\mbox{\vbox to 11pt{  \hbox{$
\int \frac{x}{ax^2+bx+c}dx  = \frac{1}{2a}\ln|ax^2+bx+c| \nonumber
\\ -\frac{b}{a\sqrt{4ac-b^2}}\tan^{-1}\frac{2ax+b}{\sqrt{4ac-b^2}}
$}  }}
\mbox{\vbox to 11pt{  \hbox{\textbf{Integrals with Roots} }  }}
\
\mbox{\vbox to 11pt{  \hbox{$
\int \frac{x}{\sqrt{x\pm a} } dx = \frac{2}{3}(x\mp 2a)\sqrt{x\pm a}
$}  }}
\
\mbox{\vbox to 11pt{  \hbox{$
\int \sqrt{\frac{x}{a-x}}dx  =  -\sqrt{x(a-x)}
%\nonumber \\ 
-a\tan^{-1}\frac{\sqrt{x(a-x)}}{x-a}
$}  }}
\
\mbox{\vbox to 11pt{  \hbox{$
\int \sqrt{\frac{x}{a+x}}dx  =  \sqrt{x(a+x)} 
%\nonumber \\  
-a\ln \left [ \sqrt{x} + \sqrt{x+a}\right] 
$}  }}
\
\mbox{\vbox to 11pt{  \hbox{$
\int  x \sqrt{x^2 \pm a^2} dx= \frac{1}{3}\left ( x^2 \pm a^2 \right)^{3/2} 
$}  }}
\
\mbox{\vbox to 11pt{  \hbox{$
\int  x \sqrt{ax + b}dx =
%\nonumber \\  
\frac{2}{15 a^2}(-2b^2+abx + 3 a^2 x^2)
\sqrt{ax+b}
$}  }}
\
\mbox{\vbox to 11pt{  \hbox{$
\int \sqrt{x(ax+b)} dx  = \frac{1}{4a^{3/2}}\left[(2ax + b)\sqrt{ax(ax+b)} \right. \nonumber
\\  \left.
-b^2 \ln \left| a\sqrt{x} + \sqrt{a(ax+b)} \right| \right ] 
$}  }}
\
\mbox{\vbox to 11pt{  \hbox{$
\int\sqrt{x^2 \pm a^2} dx  = \frac{1}{2}x\sqrt{x^2\pm a^2} 
%\nonumber \\ 
\pm\frac{1}{2}a^2 \ln \left | x + \sqrt{x^2\pm a^2} \right | 
$}  }}
\
\mbox{\vbox to 11pt{  \hbox{$
\int \sqrt{x^3(ax+b)} dx  =\left [ 
\frac{b}{12a}-
\frac{b^2}{8a^2x}+
\frac{x}{3}\right] 
\sqrt{x^3(ax+b)} \nonumber \\  + 
\frac{b^3}{8a^{5/2}}\ln \left | a\sqrt{x} + \sqrt{a(ax+b)} \right |
$}  }}
\
\mbox{\vbox to 11pt{  \hbox{$
\int  \sqrt{a^2 - x^2} dx  = \frac{1}{2} x \sqrt{a^2-x^2} 
%\nonumber \\  
+\frac{1}{2}a^2\tan^{-1}\frac{x}{\sqrt{a^2-x^2}}
$}  }}
\
\mbox{\vbox to 11pt{  \hbox{$
\int \frac{x^2}{\sqrt{x^2 \pm a^2}} dx  = \frac{1}{2}x\sqrt{x^2 \pm a^2}
%\nonumber \\  
\mp \frac{1}{2}a^2 \ln \left| x + \sqrt{x^2\pm a^2} \right | 
$}  }}
\
\mbox{\vbox to 11pt{  \hbox{$
\int \frac{1}{\sqrt{x^2 \pm a^2}} dx = \ln \left | x + \sqrt{x^2 \pm a^2} \right | 
$}  }}
\
\mbox{\vbox to 11pt{  \hbox{$
\int \frac{1}{\sqrt{a^2 - x^2}} dx = \sin^{-1}\frac{x}{a} 
$}  }}
\
\mbox{\vbox to 11pt{  \hbox{$
\int \frac{x}{\sqrt{x^2\pm a^2}}dx = \sqrt{x^2 \pm a^2} 
$}  }}
\
\mbox{\vbox to 11pt{  \hbox{$
\int \frac{x}{\sqrt{a^2-x^2}}dx = -\sqrt{a^2-x^2} 
$}  }}
\
\mbox{\vbox to 11pt{  \hbox{$
\int  \sqrt{a x^2 + b x + c} dx = 
\frac{b+2ax}{4a}\sqrt{ax^2+bx+c}
\nonumber \\  
+
\frac{4ac-b^2}{8a^{3/2}}\ln \left| 2ax + b + 2\sqrt{a(ax^2+bx^+c)}\right |
$}  }}
\
\mbox{\vbox to 11pt{  \hbox{$
\int  x \sqrt{a x^2 + bx + c} = \frac{1}{48a^{5/2}}\left ( 
2 \sqrt{a} \sqrt{ax^2+bx+c}
\right . \nonumber \\   
 \times \left( -3b^2 + 2 abx + 8 a(c+ax^2) \right)
 \nonumber \\   \left.
 + 3(b^3-4abc)\ln \left|b + 2ax + 2\sqrt{a}\sqrt{ax^2+bx+c} \right| \right)
$}  }}
\
\mbox{\vbox to 11pt{  \hbox{$
\int \frac{1}{\sqrt{ax^2+bx+c}}dx=
%==\nonumber \\ 
\frac{1}{\sqrt{a}}\ln \left| 2ax+b + 2 \sqrt{a(ax^2+bx+c)} \right | 
$}  }}
\
\mbox{\vbox to 11pt{  \hbox{$
\int  \frac{x}{\sqrt{ax^2+bx+c}}dx=
\frac{1}{a}\sqrt{ax^2+bx + c} \nonumber \\ 
-
\frac{b}{2a^{3/2}}\ln \left| 2ax+b + 2 \sqrt{a(ax^2+bx+c)} \right |
$}  }}
\
\mbox{\vbox to 11pt{  \hbox{$
\int\frac{dx}{(a^2+x^2)^{3/2}}=\frac{x}{a^2\sqrt{a^2+x^2}}
$}  }}
\
\mbox{\vbox to 11pt{  \hbox{\textbf{Integrals with Logarithms} }  }}
\
\mbox{\vbox to 11pt{  \hbox{$
\int \ln (ax + b) dx = \left ( x + \frac{b}{a} \right) \ln (ax+b) - x , a\ne 0
$}  }}
\
\mbox{\vbox to 11pt{  \hbox{$
\int \frac{\ln ax}{x} dx = \frac{1}{2}\left ( \ln ax \right)^2 
$}  }}
\
\mbox{\vbox to 11pt{  \hbox{$
\int \ln  ( x^2 + a^2 )\hspace{.5ex}\text{dx} = x \ln (x^2 + a^2  ) +2a\tan^{-1} \frac{x}{a} - 2x 
$}  }}
\
\mbox{\vbox to 11pt{  \hbox{$
\int \ln  ( x^2 - a^2 )\hspace{.5ex}\text{dx} = x \ln (x^2 - a^2  ) +a\ln \frac{x+a}{x-a} - 2x $}  }}
\
\mbox{\vbox to 11pt{  \hbox{$
\int x \ln (ax + b) dx  = \frac{bx}{2a}-\frac{1}{4}x^2 \nonumber
\\ 
+\frac{1}{2}\left(x^2-\frac{b^2}{a^2}\right)\ln (ax+b) 
$}  }}
\
\mbox{\vbox to 11pt{  \hbox{$
\int \ln   \left ( ax^2 + bx + c\right) dx  = \frac{1}{a}\sqrt{4ac-b^2}\tan^{-1}\frac{2ax+b}{\sqrt{4ac-b^2}}
\nonumber \\   -2x
 + \left( \frac{b}{2a}+x \right )\ln \left (ax^2+bx+c \right) 
$}  }}
\
\mbox{\vbox to 11pt{  \hbox{$
\int x \ln \left ( a^2 - b^2 x^2 \right ) dx  = -\frac{1}{2}x^2+ \nonumber
\\ 
\frac{1}{2}\left( x^2 - \frac{a^2}{b^2} \right ) \ln \left (a^2 -b^2 x^2 \right) 
$}  }}
\
\mbox{\vbox to 11pt{  \hbox{\textbf{Integrals with Exponentials} }  }}
\
\mbox{\vbox to 11pt{  \hbox{$
\int x^n e^{ax}\hspace{1pt}\text{d}x = \dfrac{x^n e^{ax}}{a} - 
\dfrac{n}{a}\int x^{n-1}e^{ax}\hspace{1pt}\text{d}x
$}  }} 
\
\mbox{\vbox to 11pt{  \hbox{$
\int x e^{-ax^2}\ \text{dx} = -\dfrac{1}{2a}e^{-ax^2} 
$}  }}
\
\mbox{\vbox to 11pt{  \hbox{\textbf {Integrals with Trigonometric Functions} }  }}
\
\mbox{\vbox to 11pt{  \hbox{$
\int \sin^3 ax dx = -\frac{3 \cos ax}{4a} + \frac{\cos 3ax} {12a} 
$}  }}
\
\mbox{\vbox to 11pt{  \hbox{$
\int \cos^2 ax dx = \frac{x}{2}+\frac{ \sin 2ax}{4a} 
$}  }}
\
\mbox{\vbox to 11pt{  \hbox{$
\int \cos^3 ax dx = \frac{3 \sin ax}{4a}+\frac{ \sin 3ax}{12a} 
$}  }}
\
\mbox{\vbox to 11pt{  \hbox{$
\int \cos ax \sin bx dx  = \frac{\cos[(a-b) x]}{2(a-b)} -
%\nonumber \\  
 \frac{\cos[(a+b)x]}{2(a+b)} , a\ne b
$}  }}
\
\mbox{\vbox to 11pt{  \hbox{$
\int \sin^2 ax \cos bx dx  = 
-\frac{\sin[(2a-b)x]}{4(2a-b)} \nonumber \\   
+ \frac{\sin bx}{2b} 
- \frac{\sin[(2a+b)x]}{4(2a+b)}
$}  }}
\
\mbox{\vbox to 11pt{  \hbox{$
\int \sin^2 x \cos x dx = \frac{1}{3} \sin^3 x
$}  }}
\
\mbox{\vbox to 11pt{  \hbox{$
\int \cos^2 ax \sin bx dx  = \frac{\cos[(2a-b)x]}{4(2a-b)} 
- \frac{\cos bx}{2b}
\nonumber \\  
 - \frac{\cos[(2a+b)x]}{4(2a+b)}
$}  }}
\
\mbox{\vbox to 11pt{  \hbox{$
\int \cos^2 ax \sin ax dx = -\frac{1}{3a}\cos^3{ax} 
$}  }}
\
\mbox{\vbox to 11pt{  \hbox{$
\int \sin^2 ax \cos^2 bx dx  = \frac{x}{4}
-\frac{\sin 2ax}{8a}-
\frac{\sin[2(a-b)x]}{16(a-b)}
\nonumber \\  
+\frac{\sin 2bx}{8b}-
\frac{\sin[2(a+b)x]}{16(a+b)}
$}  }}
\
\mbox{\vbox to 11pt{  \hbox{$
\int \sin^2 ax \cos^2 ax dx = \frac{x}{8}-\frac{\sin 4ax}{32a}
$}  }}
\
\mbox{\vbox to 11pt{  \hbox{$
\int \tan ax dx = -\frac{1}{a} \ln \cos ax 
$}  }}
\
\mbox{\vbox to 11pt{  \hbox{$
\int \tan^2 ax dx = -x + \frac{1}{a} \tan ax 
$}  }}
\
\mbox{\vbox to 11pt{  \hbox{$
\int \tan^3 ax dx = \frac{1}{a} \ln \cos ax + \frac{1}{2a}\sec^2 ax 
$}  }}
\
\mbox{\vbox to 11pt{  \hbox{$
\int \sec x dx  = \ln | \sec x + \tan x | = 2 \tanh^{-1} \left (\tan \frac{x}{2} \right) 
$}  }}
\
\mbox{\vbox to 11pt{  \hbox{$
\int \sec^2 ax dx = \frac{1}{a} \tan ax 
$}  }}
\
\mbox{\vbox to 11pt{  \hbox{$
\int \sec^3 x \hspace{2pt}\text{dx} = \frac{1}{2} \sec x \tan x + \frac{1}{2}\ln | \sec x + \tan x |
$}  }}
\
\mbox{\vbox to 11pt{  \hbox{$
\int \sec x \tan x dx = \sec x 
$}  }}
\
\mbox{\vbox to 11pt{  \hbox{$
\int \sec^2 x \tan x dx = \frac{1}{2} \sec^2 x 
$}  }}
\
\mbox{\vbox to 11pt{  \hbox{$
\int \sec^n x \tan x dx = \frac{1}{n} \sec^n x , n\ne 0
$}  }}
\
\mbox{\vbox to 11pt{  \hbox{$
\int \csc x dx = \ln \left | \tan \frac{x}{2} \right|  = \ln | \csc x - \cot x| + C
$}  }}
\
\mbox{\vbox to 11pt{  \hbox{$
\int \csc^2 ax dx = -\frac{1}{a} \cot ax 
$}  }}
\
\mbox{\vbox to 11pt{  \hbox{$
\int \csc^3 x dx = -\frac{1}{2}\cot x \csc x + \frac{1}{2} \ln | \csc x - \cot x | 
$}  }}
\
\mbox{\vbox to 11pt{  \hbox{$
\int \csc^nx \cot x dx = -\frac{1}{n}\csc^n x, n\ne 0
$}  }}
\
\mbox{\vbox to 11pt{  \hbox{$
\int \sec x \csc x dx = \ln | \tan x | 
$}  }}
\
\mbox{\vbox to 11pt{  \hbox{\textbf{Products of Trigonometric Functions and Monomials} }  }}
\
\mbox{\vbox to 11pt{  \hbox{$
\int x \cos x dx = \cos x + x \sin x 
$}  }}
\
\mbox{\vbox to 11pt{  \hbox{$
\int x \cos ax dx = \frac{1}{a^2} \cos ax + \frac{x}{a} \sin ax 
$}  }}
\
\mbox{\vbox to 11pt{  \hbox{$
\int x^2 \cos x dx = 2 x \cos x + \left ( x^2 - 2 \right ) \sin x 
$}  }}
\
\mbox{\vbox to 11pt{  \hbox{$
\int x^2 \cos ax dx = \frac{2 x \cos ax }{a^2} + \frac{ a^2 x^2 - 2  }{a^3} \sin ax 
$}  }}
\
\mbox{\vbox to 11pt{  \hbox{$
\int x \sin x dx = -x \cos x + \sin x 
$}  }}
\
\mbox{\vbox to 11pt{  \hbox{$
\int x \sin ax dx = -\frac{x \cos ax}{a} + \frac{\sin ax}{a^2} 
$}  }}
\
\mbox{\vbox to 11pt{  \hbox{$
\int x^2 \sin x dx = \left(2-x^2\right) \cos x + 2 x \sin x
$}  }}
\
\mbox{\vbox to 11pt{  \hbox{$
\int x^2 \sin ax dx =\frac{2-a^2x^2}{a^3}\cos ax +\frac{ 2 x \sin ax}{a^2} 
$}  }}
\
\mbox{\vbox to 11pt{  \hbox{\textbf{Products of Trigonometric Functions and Exponentials} }  }}
\
\mbox{\vbox to 11pt{  \hbox{$
\int e^x \sin x dx = \frac{1}{2}e^x (\sin x - \cos x) 
$}  }}
\
\mbox{\vbox to 11pt{  \hbox{$
\int e^{bx} \sin ax dx = \frac{1}{a^2+b^2}e^{bx} (b\sin ax - a\cos ax) 
$}  }}
\
\mbox{\vbox to 11pt{  \hbox{$
\int e^{bx} \cos ax dx = \frac{1}{a^2 + b^2} e^{bx} ( a \sin ax + b \cos ax ) 
$}  }}
\
\mbox{\vbox to 11pt{  \hbox{$
\int x e^x \sin x dx = \frac{1}{2}e^x (\cos x - x \cos x + x \sin x) 
$}  }}
\
\mbox{\vbox to 11pt{  \hbox{$
\int x e^x \cos x dx = \frac{1}{2}e^x (x \cos x 
- \sin x + x \sin x) 
$}  }}
\
\mbox{\vbox to 11pt{  \hbox{$
\int e^x \cos x dx = \frac{1}{2}e^x (\sin x + \cos x)  
$}  }}
\
  }
}
\end{footnotesize}
